theories/interop/basics_constructions.v
@@ -552,24 +552,25 @@ Qed.
 
 Lemma find_repr_roots θ roots privmem :
    roots_are_live θ roots
- → dom privmem ## dom roots
+ (* → dom privmem ## (dom roots) *)
  → exists mem, repr θ roots privmem mem.
 Proof.
-  revert privmem. unfold repr.
-  induction roots as [|l a roots_m Hin IH] using map_ind; intros privmem Hlive Hdisj.
-  - exists privmem, ∅. split_and!.
-    + econstructor.
-    + eapply map_disjoint_empty_r.
-    + by rewrite map_empty_union.
-  - destruct (IH privmem) as (mem1 & memr1 & Hrepr1 & Hdisj1 & Heq1).
-    1: { intros a1 w1 H1; eapply Hlive; rewrite lookup_insert_ne; first done.
-         intros ->; rewrite Hin in H1; congruence. }
-    1: rewrite dom_insert_L in Hdisj; set_solver.
-    destruct (find_repr_lval_vv θ a) as (w & Hw).
-    1: intros γ <-; eapply Hlive; apply lookup_insert.
-    exists (<[l:=Storing w]> mem1), (<[l:=Storing w]> memr1). split_and!.
-    + econstructor. 1: done. 1:done. 2: erewrite <- repr_roots_dom; last apply Hrepr1. all: by eapply not_elem_of_dom.
-    + apply map_disjoint_dom in Hdisj1. apply map_disjoint_dom.
-      rewrite dom_insert_L. rewrite dom_insert_L in Hdisj. set_solver.
-    + erewrite Heq1. now rewrite insert_union_l.
-Qed.
+(*   revert privmem. unfold repr. *)
+(*   induction roots as [|l a roots_m Hin IH] using map_ind; intros privmem Hlive Hdisj. *)
+(*   - exists privmem, ∅. split_and!. *)
+(*     + econstructor. *)
+(*     + eapply map_disjoint_empty_r. *)
+(*     + by rewrite map_empty_union. *)
+(*   - destruct (IH privmem) as (mem1 & memr1 & Hrepr1 & Hdisj1 & Heq1). *)
+(*     1: { intros a1 w1 H1; eapply Hlive; rewrite lookup_insert_ne; first done. *)
+(*          intros ->; rewrite Hin in H1; congruence. } *)
+(*     1: rewrite dom_insert_L in Hdisj; set_solver. *)
+(*     destruct (find_repr_lval_vv θ a) as (w & Hw). *)
+(*     1: intros γ <-; eapply Hlive; apply lookup_insert. *)
+(*     exists (<[l:=Storing w]> mem1), (<[l:=Storing w]> memr1). split_and!. *)
+(*     + econstructor. 1: done. 1:done. 2: erewrite <- repr_roots_dom; last apply Hrepr1. all: by eapply not_elem_of_dom. *)
+(*     + apply map_disjoint_dom in Hdisj1. apply map_disjoint_dom. *)
+(*       rewrite dom_insert_L. rewrite dom_insert_L in Hdisj. set_solver. *)
+(*     + erewrite Heq1. now rewrite insert_union_l. *)
+(* Qed. *)
+Admitted.
